\documentclass[12pt]{extarticle}
\usepackage[a3paper,twoside,margin={0.25cm,1.3cm}]{geometry}
\usepackage[latin1]{inputenc}
\usepackage[english]{babel}
\usepackage{multicol, fancyhdr}
\usepackage{amsbsy, amssymb, amsmath, gensymb}
\usepackage[usenames,dvipsnames]{color}
\usepackage{graphicx}
\pagestyle{fancy}

\rhead{{Jens Wir\'{e}n} $<$\href{mailto:jenswir@kth.se}{jenswir@kth.se}$>$ \today}
\lhead{Formulas in Condensed Matter Theory SI2600 KTH}

\title{Formulas in Condensed Matter Theory}
\author{Jens Wir\'{e}n $<$jenswir@kth.se$>$}

\definecolor{DarkBlue}{rgb}{0,0,0.4}
\definecolor{DarkRed}{rgb}{0.6,0,0}
\usepackage[bookmarks=true]{hyperref}
\hypersetup{
  pdfauthor={Several},%
  pdftitle={Formulas in Condensed Matter Theory}%
}
\hypersetup{
  colorlinks,%
  urlcolor=DarkBlue,%
  linkcolor=DarkRed%
}

%Average
\newcommand{\average}[1]{\ensuremath{\left\langle #1 \right\rangle}}
%Parenthesis 
\newcommand{\parentheses}[1]{\ensuremath{\left( #1 \right)}}
%Absolute value
\newcommand{\absolutevalue}[1]{\ensuremath{\left| #1 \right|}}
%Commutator
\newcommand{\commutator}[1]{\ensuremath{\left[ #1 \right]}}
%Anti-commutator
\newcommand{\anticommutator}[1]{\ensuremath{\left\lbrace #1 \right\rbrace}}
%QED
\newcommand{\QED}{\begin{flushright}\textit{Q.E.D.}\end{flushright}}
%Split
\newcommand{\spliteq}[1]{\begin{split} #1 \end{split}}
%ket
\newcommand{\ket}[1]{\left| #1 \right\rangle}
%bra
\newcommand{\bra}[1]{\left\langle #1 \right|}
%\braket
\newcommand{\braket}[2]{\left\langle #1 \; \right| \left. #2 \right\rangle}
%creation operator
\newcommand{\creation}[1]{\hat{#1}^{\dagger}}

\newcommand{\U}[1]{\textrm{#1}}
\newcommand{\mysection}[1]{
\vspace{1mm}
\hrule
\section{\Huge{#1}}}

\begin{document}

\begin{center}
\resizebox{22 cm}{!}{Formulas in Condensed Matter Theory}
\end{center}

\begin{multicols*}{2}
\setlength{\columnseprule}{0.3pt}

\mysection{Second Quantization}
\subsection{Creation and Annihilation Operators}
$$\hat{a}=\sqrt{\dfrac{m \omega}{2}} \hat{x} + \dfrac{i}{\sqrt{2m \omega}} \hat{p}$$
$$\creation{a}=\sqrt{\dfrac{m \omega}{2}} \hat{x} - \dfrac{i}{\sqrt{2m \omega}} \hat{p}$$
$$\creation{a} \ket{n} = \sqrt{n+1}\ket{n+1}$$
$$\hat{a} \ket{n} = \sqrt{n}\ket{n-1}$$
$$\commutator{\hat{a},\creation{a}} = 1$$

\subsection{Number Operator}
$$\hat{N}= \creation{a} \hat{a}	$$
$$\commutator{\hat{N},\creation{a}} = \creation{a}$$
$$\commutator{\hat{N},\hat{a}} = -\hat{a}$$
$$\hat{H}= \omega \parentheses{\hat{N}+\dfrac{1}{2}}$$

\mysection{Crystal Structure \& Reciprocal Lattice}
$$\mathbf{T}=n_1\mathbf{a}_1+n_2\mathbf{a}_2+n_3\mathbf{a}_3$$
$$\mathbf{b}_1=2\pi \dfrac{\mathbf{a}_2\times\mathbf{a}_3}{\mathbf{a}_1 \cdot \parentheses{\mathbf{a}_2\times\mathbf{a}_3}}$$
$$\mathbf{b}_2=2\pi \dfrac{\mathbf{a}_1\times\mathbf{a}_3}{\mathbf{a}_2 \cdot \parentheses{\mathbf{a}_1\times\mathbf{a}_3}}$$
$$\mathbf{b}_3=2\pi \dfrac{\mathbf{a}_1\times\mathbf{a}_2}{\mathbf{a}_3 \cdot \parentheses{\mathbf{a}_1\times\mathbf{a}_2}}$$
$$\mathbf{G}=m_1\mathbf{b}_1+m_2\mathbf{b}_2+m_3\mathbf{b}_3$$
$$V_c^{(rcpr)}=(2\pi)^{d}/V_c$$

\mysection{Vibrations of Atoms}
\subsection{General Theory}
$$L=\sum_n \dfrac{m_n \dot{\mathbf{u}}_n^2}{2}-U \parentheses{ \anticommutator{\mathbf{R}_n} }$$
$$m_n \ddot{u}_n^i= - \sum_{nn'} A^{ii'}_{nn'} u^{i'}_{n'}$$
$$A^{ik}_{nn'}=\dfrac{1}{2} \parentheses{\dfrac{\partial^2 U}{\partial R^i_n R^{i'}_{n'}} +\dfrac{\partial^2 U}{\partial R^{i'}_{n'} R^i_n }} \big|_{\anticommutator{\mathbf{R}_n}=\anticommutator{\mathbf{R}_n^{(0)}}}$$
$$\mathbf{u}_n(t)=\dfrac{\mathbf{v}_n}{\sqrt{m_n}}e^{-i \omega t}$$
$$\omega^2 v_n^i = \sum_{n'i'} \tilde{A}_{nn'}^{ii'} v^{i'}_{n'}$$
$$\det \parentheses{\tilde{A}-\omega^2 \mathrm{I}}=0$$

\subsection{Phonons}
$$m_j \ddot{u}_{\mathbf{n}j}^i = - \sum_{\mathbf{n}'j'i'} A_{jj'}^{ii'}(\mathbf{n}-\mathbf{n}') u^{i'}_{\mathbf{n}'j'}$$
$$\mathbf{u}_{\mathbf{n}j}(t)=\mathbf{u}_j(\mathbf{q},t) e^{i \mathbf{q} \cdot \mathbf{T}_\mathbf{n}}$$
$$m_j \ddot{u}_{j}^i (\mathbf{q}) = - \sum_{'j'i'} C_{jj'}^{ii'}(\mathbf{q}) u^{i'}_{'j'}(\mathbf{q})$$
$$C_{jj'}^{ii'}(\mathbf{q})=\sum_{\mathbf{n}_1'j'i'} A_{jj'}^{ii'}(\mathbf{n}_1) e^{-i \mathbf{q} \cdot \mathbf{T}_{\mathbf{n}_1}}$$
$$\sum_{\beta=1}^{d\nu_0} \tilde{C}_{\alpha \beta} v_{\beta} = \omega^ 2 v_{\alpha}$$
$$\det \parentheses{\tilde{C}(\mathbf{q})-\omega^2(\mathbf{q}) \mathrm{I}}=0$$

\subsection{Therodynamics of Phonons}
$$H_{ph}= \sum_{\nu \mathbf{q}} \epsilon_{\nu \mathbf{q}} \parentheses{\creation{b}_{\nu \mathbf{q}} \hat{b}_{\nu \mathbf{q}} + \dfrac{1}{2}}$$
$$Z= \mathrm{Tr} \; e^{-H/T}$$
$$F=-T \ln Z$$
$$D(\epsilon)=\sum_{\nu \mathbf{q}} \delta \parentheses{\epsilon - \epsilon_{\nu \mathbf{q}}}$$
$$F=T \int d\epsilon D(\epsilon) \ln \parentheses{1-e^{-\epsilon/T}}$$
$$S = -\parentheses{\dfrac{\partial F}{\partial T}}_{V}$$
$$E = F + TS$$
$$C_V = \parentheses{\dfrac{\partial E}{\partial T}}_{V}$$
$$E= \int d\epsilon D(\epsilon) \epsilon n_{\epsilon}$$
$$n_{\epsilon}=\dfrac{1}{e^{\epsilon/T}-1}$$
$$N_{bosons}= \int d\epsilon D(\epsilon) n_{\epsilon}$$

\subsection{Quantum Theory of Phonons}
$$\average{\hat{b}_{\nu \mathbf{g}}}=\average{\creation{b}_{\nu \mathbf{g}}}=0 \Longrightarrow \average{\mathbf{u}_{\mathbf{n}j}}=0$$
$$\average{\mathbf{u}_{\mathbf{n}j}^2} \propto \average{\creation{b}_{sj} \hat{b}_{si}}$$
$$\average{\parentheses{\mathbf{u}_{\mathbf{n}j}^i}^2} = \dfrac{1}{m_j}\sum_\nu \int_{BZ} \dfrac{d^dg}{(2\pi)^d} \absolutevalue{v_{j\nu}^i(\mathbf{g})}^2 \dfrac{\bar{n}_{\nu \mathbf{g}}+1/2}{\omega_\nu (\mathbf{g})}$$
$$\bar{n}_{\nu \mathbf{g}} \equiv \average{n_{\nu \mathbf{g}}}=\dfrac{1}{e^{\omega_\nu (\mathbf{g})/T}-1}$$
$$\average{\parentheses{\mathbf{u}_{\mathbf{n}j}^i}^2} \sim [\mathrm{non-singular \; part]} + T \int_0^{cutoff} \dfrac{dg}{g^{3-d}} \rightarrow \infty \qquad \parentheses{d \leq 2, \: T > 0}$$
$$\average{\parentheses{\mathbf{u}_{\mathbf{n}j}^i}^2} \sim [\mathrm{non-singular \; part]} + T \int_0^{cutoff} \dfrac{dg}{g} \rightarrow \infty \qquad \parentheses{d = 1, \: T = 0}$$

\mysection{Electronic Subsystem}
\subsection{Bloch's Theory}
$$H= H_{kin}+U(\mathbf{r})$$
$$H_{kin}= -\dfrac{\nabla^ 2}{2m}$$
$$U(\mathbf{r}+\mathbf{T})=U(\mathbf{r})$$
$$\psi_{\nu \mathbf{q}}(\mathbf{r)}= u_{\nu \mathbf{q}}(\mathbf{r)} e^{i \mathbf{q} \cdot \mathbf{r}}$$
$$u_{\nu \mathbf{q}}(\mathbf{r)} = \sum_{\mathbf{G}} f_\nu \parentheses{\mathbf{q}+\mathbf{G}} e^{i \mathbf{G} \cdot \mathbf{r}}$$
$$u_{\nu \mathbf{q}}(\mathbf{r}+\mathbf{T}) = u_{\nu \mathbf{q}}(\mathbf{r)}$$
$$(H-E)\psi=0$$
$$\psi=\sum_{\mathbf{q}}C_{\mathbf{q}}e^{i \mathbf{q}\cdot \mathbf{r}}$$
$$H_{kin} e^{i \mathbf{q}\cdot \mathbf{r}} = E^{(0)e^{i \mathbf{q}\cdot \mathbf{r}}}$$
$$E^{(0)}(\mathbf{q})=\dfrac{q^2}{2m}$$

\subsection{Eigenvalue Repulsion}
$$\det \parentheses{M-\lambda \mathrm{I}}=0$$
$$\lambda_{\nu_1}(p_*)=\lambda_{\nu_2}(p_*)$$
$$\det \parentheses{M-\lambda \mathrm{I}}=(\lambda_{\nu_1}-\lambda)(\lambda_{\nu_2}-\lambda)f(\lambda), \; (p=p_*)$$
$$P=(\lambda_{\nu_1}-\lambda)(\lambda_{\nu_2}-\lambda)=\lambda^2-2b\lambda+c$$
$$\lambda_{1,2}=b\pm \sqrt{b^2-c}$$

\subsection{Wannier Functions}
$$\Phi_{\nu \mathbf{n}}(\mathbf{r})=\dfrac{1}{\sqrt{N}} \sum_{\mathbf{q}}^{BZ} e^{-i \mathbf{q} \cdot \mathbf{T}_{\mathbf{n}}} \psi_{\nu \mathbf{q}}(\mathbf{r})$$
$$\ket{\Phi_{\mathbf{n}}} \sum_{\mathbf{q}} U_{\mathbf{nq}} \ket{\psi_{\mathbf{q}}}$$
$$U_{\mathbf{nq}}=\dfrac{1}{\sqrt{N}}e^{-i \mathbf{q} \cdot \mathbf{T}_{\mathbf{n}}}$$
$$U^\dagger U = U U^\dagger = 1$$
$$\Phi_{0}(\mathbf{r}) \equiv \Phi_{\mathbf{n=0}}(\mathbf{r})$$
$$\Phi_{\mathbf{n}}(\mathbf{r})=\Phi_{0}(\mathbf{r}-\mathbf{T_{n}})$$
$$\Phi_{\mathbf{n}}(\mathbf{r})= \dfrac{1}{N}\sum_{\mathbf{q}}^{BZ} e^{i \mathbf{q} \cdot (\mathbf{r}-\mathbf{T_{n}})} u_{\mathbf{q}}(\mathbf{r})= \dfrac{1}{N}\sum_{\mathbf{q}}^{BZ} e^{i \mathbf{q} \cdot (\mathbf{r}-\mathbf{T_{n}})} u_{\mathbf{q}}(\mathbf{r}-\mathbf{T_n})$$
$$\Phi_{0}(\mathbf{r})=\dfrac{V_0}{(2\pi)^d} \int_{BZ} e^{i \mathbf{q} \cdot \mathbf{r}} u_{\mathbf{q}}(\mathbf{r}) d^dq, \quad (N \rightarrow \infty)$$

\subsection{Hopping Hamiltonian}
$$H= \sum_{\mathbf{q}} E(\mathbf{q}) \creation{a}_{\mathbf{q}} \hat{a}_{\mathbf{q}}$$
$$\hat{a}_{\mathbf{q}}= \dfrac{1}{\sqrt{N}} \sum_{\mathbf{n}} e^{-i \mathbf{q} \cdot \mathbf{T_n}} \hat{a}_{\mathbf{n}}$$
$$\hat{a}_{\mathbf{n}}= \dfrac{1}{\sqrt{N}} \sum_{\mathbf{q}} e^{i \mathbf{q} \cdot \mathbf{T_n}} \hat{a}_{\mathbf{q}}$$
$$\creation{a}_{\mathbf{q}}= \dfrac{1}{\sqrt{N}} \sum_{\mathbf{n}} e^{i \mathbf{q} \cdot \mathbf{T_n}} \creation{a}_{\mathbf{n}}$$
$$\creation{a}_{\mathbf{n}}= \dfrac{1}{\sqrt{N}} \sum_{\mathbf{q}} e^{-i \mathbf{q} \cdot \mathbf{T_n}} \creation{a}_{\mathbf{q}}$$
$$H=- \sum_{\mathbf{n},\mathbf{m}}  t_{\mathbf{m}} \: \creation{a}_{\mathbf{n+m}} a_{\mathbf{n}}$$
$$t_{\mathbf{m}}=-\dfrac{V_0}{(2\pi)^d}\int_{BZ} E(\mathbf{q}) e^{i \textbf{q} \cdot \mathbf{T_m}} d^dq$$
$$E(\mathbf{q})= -\sum_{\mathbf{m}} t_{\mathbf{m}} e^{-i \mathbf{q} \cdot \mathbf{T_m}}$$

\subsection{Tight-Binding Limit}
$$H= -t \sum_{\average{i,j}} \creation{a}_{j} \hat{a}_{i}$$
$$E(\mathbf{q})= -t\sum_{\mathbf{m}}^{n.n.} e^{-i \mathbf{q} \cdot \mathbf{T_m}}$$
$$H=- \sum_{\mathbf{n},\mathbf{m}, \alpha, \beta}  t_{\alpha, \beta}(\mathbf{m}) \: \creation{a}_{\alpha(\mathbf{n+m})} a_{\beta \mathbf{n}}$$
$$\hat{a}_{\alpha\mathbf{n}}= \dfrac{1}{\sqrt{N}} \sum_{\mathbf{q}} e^{i \mathbf{q} \cdot \mathbf{T_n}} \hat{a}_{\alpha\mathbf{q}}$$
$$\creation{a}_{\alpha\mathbf{n}}= \dfrac{1}{\sqrt{N}} \sum_{\mathbf{q}} e^{-i \mathbf{q} \cdot \mathbf{T_n}} \creation{a}_{\alpha\mathbf{q}}$$
$$H=\sum_{\mathbf{q}} \sum_{\alpha, \beta} H_{\alpha \beta}(\mathbf{q}) \creation{a}_{\alpha \mathbf{q}} \hat{a}_{\beta \mathbf{q}}$$
$$H_{\alpha \beta}(\mathbf{q})= -\sum_{\mathbf{m}} t_{\alpha \beta}(\mathbf{m}) e^{-i \mathbf{q} \cdot \mathbf{T_m}}$$
$$\sum_{\beta} H_{\alpha \beta} u_{\beta}^{(\nu)}= E_{\nu} u_{\alpha}^{(\nu)}$$
$$\creation{a}_{\alpha}=\sum_{\nu} \commutator{u_{\alpha}^{(\nu)}}^* \creation{b}_{\nu}$$
$$\hat{a}_{\beta}=\sum_{\nu} u_{\alpha}^{(\nu)} \hat{b}_{\nu}$$
$$H=\sum_{\nu \mathbf{q}} E_{\nu} (\mathbf{q}) \creation{b}_{\nu \mathbf{q}} \hat{b}_{\nu \mathbf{q}}$$

\mysection{Superfluidity}

\subsection{Superfluid Velocity and its Quantum}
$$\mathbf{v}_s (\mathbf{r}) = \gamma \nabla \mathbf{\Phi (r)}$$
$$\psi = \absolutevalue{\psi} e^{i \Phi}$$
$$\partial^\mu \partial_{\mu} \psi= -\lambda^2 \psi, \quad (\gamma=c^2/\lambda)$$
$$i \dfrac{\partial \psi}{\partial t}= -\dfrac{\gamma}{2} \nabla^2 \psi$$
$$H=\dfrac{1}{2} \gamma \absolutevalue{\nabla \psi}^2 + V(\mathbf{r}) \absolutevalue{\psi}^2 + \dfrac{g}{2}\absolutevalue{\psi}^4 - \mu \absolutevalue{\psi}^2$$
$$i \dot{\psi} = -\dfrac{\gamma}{2} \nabla \psi + g \absolutevalue{\psi}^2 \psi + V(\mathbf{r}) \psi - \mu \psi$$
$$\oint \mathbf{v_s} \cdot d\mathbf{l} = \gamma \oint \nabla \Phi \cdot d\mathbf{l} \Rightarrow \absolutevalue{v_s}=\dfrac{\gamma}{r}N, \quad \parentheses{\gamma=\dfrac{\hbar}{m}}$$
$$l_0=\sqrt{\dfrac{\gamma}{g n_0}}, \quad \parentheses{\l_0 \rightarrow \infty, g \rightarrow 0}$$

\subsection{Superfluid Vortex Solution}
$$M= \dfrac{1}{2\pi} \oint_C \nabla \Phi \cdot d\mathbf{l} \neq 0$$
$$\psi(\rho, r) = \sqrt{n(\rho)} e^{\pm i \Phi}$$
$$E_{vortex}=\pi \gamma n_0 \ln \dfrac{R}{l_0}$$
$$\Delta E - MW < 0$$
$$W_c = \dfrac{\gamma}{R^2} \ln \dfrac{R}{l_0}$$

\mysection{Superconductivity}

\subsection{Gauge Tranformations}
\subsubsection{GPE}
$$\psi \mapsto \psi'=\psi e^{i \varphi}$$
$$A \mapsto A'=A-\nabla \varphi$$
$$V \mapsto V'=V+\varphi$$

\subsection{GL}
$$\psi \mapsto \psi'=\psi e^{-i \chi(\textbf{x})}$$
$$A_\mu \mapsto A'_\mu=A_\mu-\dfrac{1}{e}\nabla \chi(\textbf{x})$$

\subsubsection{QED}
$$\psi \mapsto \psi'=\psi e^{-i \alpha(x)}$$
$$A_\mu \mapsto A'_\mu=A_\mu-\dfrac{1}{e}\partial_\mu \alpha(x)$$

\subsection{Meissner Effect}
$$\lambda = \dfrac{1}{\sqrt{q\gamma n_s}}, \quad \mu_A = \lambda^{-1}$$
$$\mathbf{B} + \lambda^2 \nabla \times \nabla \times \mathbf{B} = 0$$
$$\mathbf{B}(x)=B(x) \hat{e}_z \Rightarrow B(x)=B(0) e^{-x/\lambda} \quad (x>0)$$
$$\mathbf{J}= \nabla \times \mathbf{B} \Rightarrow J_y(x)=-\dfrac{dB}{dx}=\dfrac{B(0)}{\lambda} e^{-x/\lambda} \quad (x>0)$$

\subsection{Magnetic Flux Quantization}
$$\mathbf{J}_s=-\lambda^{-2} \parentheses{\dfrac{\hbar}{q} \nabla \theta + \mathbf{A}}$$
$$\oint_C \mathbf{A} \cdot d \mathbf{l} = \int_{S_C} \nabla \times \mathbf{A} \cdot d \mathbf{\hat{s}} =  \int_{S} \mathbf{B} \cdot d \mathbf{\hat{s}} = \Phi$$
$$\oint_C \nabla \theta \cdot d\mathbf{l} = 2\pi N$$
$$\oint_C \mathbf{J}_s + \int_{S} \mathbf{B} \cdot d \mathbf{\hat{s}} = \dfrac{2 \pi \hbar N}{q}=N \Phi_0, \quad N=0,\pm 1, \pm 2...$$

\subsection{Ginzburg-Landau Theory}
$$F=\dfrac{\gamma}{2} \absolutevalue{\parentheses{\nabla + iq\mathbf{A}} \psi }^2 - a \absolutevalue{\psi}^2 + \dfrac{b}{2} \absolutevalue{\psi}^4 + \dfrac{1}{2} \parentheses{\nabla \times \mathbf{A}}^2$$
$$\dfrac{\delta F	}{\delta \psi^*}=0, \quad \dfrac{\delta F	}{\delta \mathbf{A}}=0$$

\subsection{Critical Fields}
$$\lambda = \dfrac{1}{\sqrt{q\gamma n_s}}, \xi =  \dfrac{1}{2\sqrt{a}}$$

\subsubsection{Type 1: $\kappa=\lambda/\xi \ll 1$}
$$F(\psi=0)-F(\psi=\absolutevalue{\psi} = \dfrac{a^2}{2b}= \dfrac{H_c^2}{2}$$

\subsubsection{Type 2: $\kappa=\lambda/\xi \gg 1$}
$$ G - F_{s}^{(0)} = E_v - \Phi_0 H \rightarrow H_{c1}=\dfrac{E_v}{\Phi_0}$$
$$\parentheses{-i \nabla + q\mathbf{A}}^2 \psi = 2a \psi, \quad \absolutevalue{\psi} \rightarrow 0$$
$$H_{c2}=\dfrac{\psi_0}{4 \pi \xi^ 2}$$

\subsection{Vortices}

\subsubsection{Single Vortex}
$$\mathbf{B} + \lambda^2 \nabla \times \nabla \times \mathbf{B} = \dfrac{\Phi_0}{2\pi} \nabla \times \nabla \theta$$
$$B=\dfrac{\Phi}{2\pi \lambda^2}K_0(r/\lambda)$$
$$B(0) \approx \dfrac{\Phi}{2\pi \lambda^2}\ln(\lambda/\xi)$$
$$E_v=\dfrac{\Phi}{2} \approx\dfrac{1}{4\pi}\parentheses{\dfrac{\Phi}{\lambda}}^2 \ln \parentheses{\dfrac{\lambda}{\xi}}, \quad (\Phi=N\Phi_0)$$

\subsubsection{Vortex Interactions in the London Limit}
$$E_{tot} = NE_{v}+\sum_{r_{kl}} E_{int}(r_{kl})$$
$$F = -\dfrac{dE_{int}}{dr_{ij}}$$
$$F_{free}=\int \dfrac{\mathbf{B}}{2} \parentheses{\mathbf{B}+\dfrac{1}{e^2 \rho^2} \nabla \times \nabla \times \mathbf{B}}$$
$$\dfrac{1}{e^2 \rho^2} \nabla \times \nabla \times \mathbf{B} + \mathbf{B} = \sum_i \Phi_i \delta(\mathbf{x}-\mathbf{x}_i)$$
$$\mathbf{B}_i=\dfrac{\Phi_i e^2 \rho^2}{2\pi}K_0\parentheses{\dfrac{|\mathbf{x}-\mathbf{x}_i|}{\lambda}}$$
$$F_{free}=\int \dfrac{1}{2} \parentheses{\mathbf{B}_a+\mathbf{B}_b} \parentheses{\Phi_a \delta(\mathbf{x}-\mathbf{x}_a)+\Phi_b \delta(\mathbf{x}-\mathbf{x}_b)}=$$
$$=-\dfrac{\Phi_a \Phi_b e^2 \rho^2}{2 \pi}K_0 \parentheses{\dfrac{r}{\lambda}} + E_{\nu a}+ E_{\nu b}$$
$$r_{ij}=|\mathbf{x}_2-\mathbf{x}_1|$$
$$E_{int,aa}=-\dfrac{|\psi_a|^4}{\rho^2}K_0 \parentheses{\dfrac{r_{ij}}{\lambda}}$$
$$E^{(int),elec}_{ab}=2\pi C_1^2 K_0 \parentheses{\dfrac{\absolutevalue{\mathbf{x}_a-\mathbf{x}_b}}{\lambda}}$$
$$E^{(int),cores}_{ab}=-2\pi C_2^2 K_0 \parentheses{\dfrac{\absolutevalue{\mathbf{x}_a-\mathbf{x}_b}}{\xi}}$$
$$E^{(int)}_{ab}=2\pi \parentheses{C_1^2 K_0 \parentheses{\dfrac{d}{\lambda}}-C_2^2 K_0 \parentheses{\dfrac{d}{\xi}}}, \quad d=\absolutevalue{\mathbf{x}_a-\mathbf{x}_b}$$


\mysection{BCS-theory}
$$\omega_D - \epsilon_F < E < \omega_D + \epsilon_F$$
$$H=\sum_{\mathbf{k},\sigma} \epsilon_{\mathbf{k}} \creation{c}_{\mathbf{k}\sigma} \hat{c}_{\mathbf{k}\sigma} - \absolutevalue{g_{eff}}^2 \sum \creation{c}_{\mathbf{k}_1+\mathbf{q}\sigma_1} \creation{c}_{\mathbf{k}_2-\mathbf{q}\sigma_2}  \hat{c}_{\mathbf{k}_1\sigma_1} \hat{c}_{\mathbf{k}_2\sigma_2}$$
$$H=\sum_{\mathbf{k},\sigma} \epsilon_{\mathbf{k}} \creation{c}_{\mathbf{k}\sigma} \hat{c}_{\mathbf{k}\sigma} - \absolutevalue{g_{eff}}^2 \sum_{\mathbf{k,k'}} \creation{c}_{\mathbf{k}\uparrow} \creation{c}_{-\mathbf{k}\downarrow}  \hat{c}_{-\mathbf{k}'\downarrow} \hat{c}_{\mathbf{k}'\uparrow}$$


\subsection{BCS Gap}
$$\Delta_0= \dfrac{1}{D(\epsilon_F)V} \int_0^{\omega_D} \dfrac{d \xi}{\sqrt{\xi^2 + \Delta^2_0}} \tanh \parentheses{\dfrac{\sqrt{\xi^2 + \Delta^2_0}}{2T}} \approx 2 \omega_D e^{-\dfrac{1}{D(\epsilon_F)V}}$$

\subsection{Critical Velocity}
$$\mathbf{k_F} \mapsto \mathbf{kF}+\dfrac{1}{2}\mathbf{k} \Rightarrow \Delta E = \dfrac{1}{m}k_F k$$
$$2 \Delta (T) = \dfrac{k_F k}{m} \Rightarrow p_c = \dfrac{2 \Delta}{v_F}$$
$$J_c=n_s e v_c = n_s \dfrac{e \Delta (T)}{m v_F }$$

\subsection{Critical Temperature}
$$\Delta(T) \rightarrow 0, \quad T \rightarrow T_c$$
$$\Delta(T_c)=0 \Rightarrow \dfrac{1}{D(\epsilon_F)V} \int_0^{\omega_D} \dfrac{d \xi}{\xi} \tanh \parentheses{\dfrac{\xi}{2T}} \rightarrow 0$$
$$T_c = 1.14 \omega_D e^{-\dfrac{1}{D(\epsilon_F)V}} \Rightarrow T_c = \dfrac{3.52}{2} \Delta_0$$

\end{multicols*}
\end{document}